src/CIU.v
@@ -141,10 +141,47 @@ Proof.
   split; split.
   1, 3: constructor; auto.
   all: split. 1, 3: constructor; auto.
-  * intros. (* smarter pattern matching needed *)
+  * intros. assert (FSCLOSED (FCase (PCons PVar PVar) (EVar 0) inf :: F)). {
+       constructor; auto. constructor; auto. 2: repeat constructor.
+       simpl. do 2 constructor. auto. inversion H8. inversion H8.
+     }
+     specialize (H5 (FCase (PCons PVar PVar) (EVar 0) inf :: F) H8).
+     destruct H7.
+     assert (| FCase (PCons PVar PVar) (EVar 0) inf :: F, ECons e1 e2 | ↓). {
+       exists (4 + x). apply term_cons.
+       constructor; auto. constructor; auto. eapply term_case_true.
+       constructor; auto. reflexivity.
+       simpl. auto.
+     }
+     apply H5 in H9. destruct H9.
+     inversion H9; subst; try inversion_is_value.
+     inversion H14; subst; try inversion_is_value.
+     inversion H16; subst; try inversion_is_value.
+     inversion H19; subst; try inversion_is_value.
+     - simpl in H23. inversion H23. subst. simpl in H24. eexists; eassumption.
+     - apply inf_diverges in H24. contradiction.
+  * intros. assert (FSCLOSED (FCase (PCons PVar PVar) (EVar 1) inf :: F)). {
+       constructor; auto. constructor; auto. 2: repeat constructor.
+       simpl. do 2 constructor. auto. inversion H8. inversion H8.
+     }
+     specialize (H5 (FCase (PCons PVar PVar) (EVar 1) inf :: F) H8).
+     destruct H7.
+     assert (| FCase (PCons PVar PVar) (EVar 1) inf :: F, ECons e1 e2 | ↓). {
+       exists (4 + x). apply term_cons.
+       constructor; auto. constructor; auto. eapply term_case_true.
+       constructor; auto. reflexivity.
+       simpl. auto.
+     }
+     apply H5 in H9. destruct H9.
+     inversion H9; subst; try inversion_is_value.
+     inversion H14; subst; try inversion_is_value.
+     inversion H16; subst; try inversion_is_value.
+     inversion H19; subst; try inversion_is_value.
+     - simpl in H23. inversion H23. subst. simpl in H24. eexists; eassumption.
+     - apply inf_diverges in H24. contradiction.
 Qed.
 
-Theorem CIU_implies_Vrel :
+(* Theorem CIU_implies_Vrel :
   forall e1 e2, VALCLOSED e1 -> VALCLOSED e2 -> CIU e1 e2 -> CIU e2 e1 (* for comfort *)
  -> 
   forall n, Vrel n e1 e2.
@@ -154,7 +191,7 @@ Proof.
   * split. 2: split. 1-2: constructor.
     epose proof (H1 [FCase (PLit l) (ELit 0) inf] _ _).
     destruct H3. inversion H3; subst; try inversion_is_value.
-    now apply Z.eqb_eq in H11.
+    simpl in H11. break_match_hyp. now apply Z.eqb_eq in Heqb. congruence.
     now apply inf_diverges in H12.
   * epose proof (H1 [FCase (PLit l) (ELit 0) inf] _ _).
     destruct H3. inversion H3; subst; try inversion_is_value.
@@ -172,7 +209,8 @@ Proof.
     destruct H3. inversion H3; subst; try inversion_is_value.
     inversion H11.
     now apply inf_diverges in H12.
-  * admit.
+  * split. 2: split. 1-2: auto.
+    epose proof (H1 (FCase (PLit 0) (ELit 0) (EApp ))).
   * epose proof (H2 [FCase PNil (ELit 0) inf] _ _).
     destruct H3. inversion H3; subst; try inversion_is_value.
     inversion H11.
@@ -208,7 +246,52 @@ Proof.
     now apply inf_diverges in H12.
   * split. 2: split. 1-2: auto. inversion H. inversion H0. subst.
     assert (CIU e1_1 e2_1). {
-      apply CIU_eval; auto. constructor. auto.
-      split. auto. exists 0. constructor.
-    specialize (IHe1_1 e2_1 H5 H9).
-Qed.
+      apply (CIU_list_parts e1_1 e1_2 e2_1 e2_2); auto.
+      split. 2: split. 1-2: do 2 constructor; auto.
+      intros. destruct H4.
+      inversion H4; subst; try inversion_is_value.
+      inversion H13; subst; try inversion_is_value.
+      inversion H15; subst; try inversion_is_value.
+      assert (exists k, | F, VCons e1_1 e1_2 | k ↓). { eexists; eauto. } apply H1 in H7.
+      destruct H7. exists (3 + x). constructor; auto. constructor; auto. constructor; auto.
+      auto.
+   }
+   assert (CIU e1_2 e2_2). {
+      apply (CIU_list_parts e1_1 e1_2 e2_1 e2_2); auto.
+      split. 2: split. 1-2: do 2 constructor; auto.
+      intros. destruct H7.
+      inversion H7; subst; try inversion_is_value.
+      inversion H14; subst; try inversion_is_value.
+      inversion H16; subst; try inversion_is_value.
+      assert (exists k, | F, VCons e1_1 e1_2 | k ↓). { eexists; eauto. } apply H1 in H8.
+      destruct H8. exists (3 + x). constructor; auto. constructor; auto. constructor; auto.
+      auto.
+   }
+   assert (CIU e2_1 e1_1). {
+      apply (CIU_list_parts e2_1 e2_2 e1_1 e1_2); auto.
+      split. 2: split. 1-2: do 2 constructor; auto.
+      intros. destruct H8.
+      inversion H8; subst; try inversion_is_value.
+      inversion H15; subst; try inversion_is_value.
+      inversion H17; subst; try inversion_is_value.
+      assert (exists k, | F, VCons e2_1 e2_2 | k ↓). { eexists; eauto. } apply H2 in H11.
+      destruct H11. exists (3 + x). constructor; auto. constructor; auto. constructor; auto.
+      auto.
+   }
+   assert (CIU e2_2 e1_2). {
+      apply (CIU_list_parts e2_1 e2_2 e1_1 e1_2); auto.
+      split. 2: split. 1-2: do 2 constructor; auto.
+      intros. destruct H11.
+      inversion H11; subst; try inversion_is_value.
+      inversion H16; subst; try inversion_is_value.
+      inversion H18; subst; try inversion_is_value.
+      assert (exists k, | F, VCons e2_1 e2_2 | k ↓). { eexists; eauto. } apply H2 in H12.
+      destruct H12. exists (3 + x). constructor; auto. constructor; auto. constructor; auto.
+      auto.
+   }
+   do 2 rewrite <- Vrel_Fix_eq. split.
+   - apply IHe1_1; auto.
+   - apply IHe1_2; auto.
+Unshelve.
+  
+Qed. *)
